Graph/IRNodeHierarchy2.thy
@@ -1,0 +1,288 @@
+subsection \<open>Hierarchy of Nodes\<close>
+
+theory IRNodeHierarchy2
+imports IRNodes2
+begin
+
+text \<open>
+It is helpful to introduce a node hierarchy into our formalization.
+Often the GraalVM compiler relies on explicit type checks to determine
+which operations to perform on a given node, we try to mimic the same
+functionality by using a suite of predicate functions over the IRNode
+class to determine inheritance.
+
+As one would expect, the function is<ClassName>Type will be true if
+the node parameter is a subclass of the ClassName within the GraalVM compiler.
+
+These functions have been automatically generated from the compiler.
+\<close>
+
+(* Datatype with no parameters don't generate selectors *)
+fun is_EndNode :: "IRNode \<Rightarrow> bool" where
+  "is_EndNode EndNode = True" |
+  "is_EndNode _ = False"
+
+(* nodeout: isabelle-subclass *)
+fun is_ControlSinkNode :: "IRNode \<Rightarrow> bool" where
+  "is_ControlSinkNode n = ((is_ReturnNode n) \<or> (is_UnwindNode n))"
+
+fun is_AbstractMergeNode :: "IRNode \<Rightarrow> bool" where
+  "is_AbstractMergeNode n = ((is_LoopBeginNode n) \<or> (is_MergeNode n))"
+
+fun is_BeginStateSplitNode :: "IRNode \<Rightarrow> bool" where
+  "is_BeginStateSplitNode n = ((is_AbstractMergeNode n) \<or> (is_ExceptionObjectNode n) \<or> (is_LoopExitNode n) \<or> (is_StartNode n))"
+
+fun is_AbstractBeginNode :: "IRNode \<Rightarrow> bool" where
+  "is_AbstractBeginNode n = ((is_BeginNode n) \<or> (is_BeginStateSplitNode n) \<or> (is_KillingBeginNode n))"
+
+fun is_AbstractNewArrayNode :: "IRNode \<Rightarrow> bool" where
+  "is_AbstractNewArrayNode n = ((is_DynamicNewArrayNode n) \<or> (is_NewArrayNode n))"
+
+fun is_AbstractNewObjectNode :: "IRNode \<Rightarrow> bool" where
+  "is_AbstractNewObjectNode n = ((is_AbstractNewArrayNode n) \<or> (is_NewInstanceNode n))"
+
+fun is_IntegerDivRemNode :: "IRNode \<Rightarrow> bool" where
+  "is_IntegerDivRemNode n = ((is_SignedDivNode n) \<or> (is_SignedRemNode n))"
+
+fun is_FixedBinaryNode :: "IRNode \<Rightarrow> bool" where
+  "is_FixedBinaryNode n = ((is_IntegerDivRemNode n))"
+
+fun is_DeoptimizingFixedWithNextNode :: "IRNode \<Rightarrow> bool" where
+  "is_DeoptimizingFixedWithNextNode n = ((is_AbstractNewObjectNode n) \<or> (is_FixedBinaryNode n))"
+
+fun is_AbstractMemoryCheckpoint :: "IRNode \<Rightarrow> bool" where
+  "is_AbstractMemoryCheckpoint n = ((is_BytecodeExceptionNode n) \<or> (is_InvokeNode n))"
+
+fun is_AbstractStateSplit :: "IRNode \<Rightarrow> bool" where
+  "is_AbstractStateSplit n = ((is_AbstractMemoryCheckpoint n))"
+
+fun is_AccessFieldNode :: "IRNode \<Rightarrow> bool" where
+  "is_AccessFieldNode n = ((is_LoadFieldNode n) \<or> (is_StoreFieldNode n))"
+
+fun is_FixedWithNextNode :: "IRNode \<Rightarrow> bool" where
+  "is_FixedWithNextNode n = ((is_AbstractBeginNode n) \<or> (is_AbstractStateSplit n) \<or> (is_AccessFieldNode n) \<or> (is_DeoptimizingFixedWithNextNode n))"
+
+fun is_WithExceptionNode :: "IRNode \<Rightarrow> bool" where
+  "is_WithExceptionNode n = ((is_InvokeWithExceptionNode n))"
+
+fun is_ControlSplitNode :: "IRNode \<Rightarrow> bool" where
+  "is_ControlSplitNode n = ((is_IfNode n) \<or> (is_WithExceptionNode n))"
+
+fun is_AbstractEndNode :: "IRNode \<Rightarrow> bool" where
+  "is_AbstractEndNode n = ((is_EndNode n) \<or> (is_LoopEndNode n))"
+
+fun is_FixedNode :: "IRNode \<Rightarrow> bool" where
+  "is_FixedNode n = ((is_AbstractEndNode n) \<or> (is_ControlSinkNode n) \<or> (is_ControlSplitNode n) \<or> (is_FixedWithNextNode n))"
+
+fun is_FloatingGuardedNode :: "IRNode \<Rightarrow> bool" where
+  "is_FloatingGuardedNode n = ((is_PiNode n))"
+
+fun is_UnaryArithmeticNode :: "IRNode \<Rightarrow> bool" where
+  "is_UnaryArithmeticNode n = ((is_AbsNode n) \<or> (is_NegateNode n) \<or> (is_NotNode n))"
+
+fun is_UnaryNode :: "IRNode \<Rightarrow> bool" where
+  "is_UnaryNode n = ((is_UnaryArithmeticNode n))"
+
+fun is_BinaryArithmeticNode :: "IRNode \<Rightarrow> bool" where
+  "is_BinaryArithmeticNode n = ((is_AddNode n) \<or> (is_AndNode n) \<or> (is_MulNode n) \<or> (is_OrNode n) \<or> (is_SubNode n) \<or> (is_XorNode n))"
+
+fun is_BinaryNode :: "IRNode \<Rightarrow> bool" where
+  "is_BinaryNode n = ((is_BinaryArithmeticNode n))"
+
+fun is_PhiNode :: "IRNode \<Rightarrow> bool" where
+  "is_PhiNode n = ((is_ValuePhiNode n))"
+
+fun is_IntegerLowerThanNode :: "IRNode \<Rightarrow> bool" where
+  "is_IntegerLowerThanNode n = ((is_IntegerLessThanNode n))"
+
+fun is_CompareNode :: "IRNode \<Rightarrow> bool" where
+  "is_CompareNode n = ((is_IntegerEqualsNode n) \<or> (is_IntegerLowerThanNode n))"
+
+fun is_BinaryOpLogicNode :: "IRNode \<Rightarrow> bool" where
+  "is_BinaryOpLogicNode n = ((is_CompareNode n))"
+
+fun is_UnaryOpLogicNode :: "IRNode \<Rightarrow> bool" where
+  "is_UnaryOpLogicNode n = ((is_IsNullNode n))"
+
+fun is_LogicNode :: "IRNode \<Rightarrow> bool" where
+  "is_LogicNode n = ((is_BinaryOpLogicNode n) \<or> (is_LogicNegationNode n) \<or> (is_ShortCircuitOrNode n) \<or> (is_UnaryOpLogicNode n))"
+
+fun is_ProxyNode :: "IRNode \<Rightarrow> bool" where
+  "is_ProxyNode n = ((is_ValueProxyNode n))"
+
+fun is_AbstractLocalNode :: "IRNode \<Rightarrow> bool" where
+  "is_AbstractLocalNode n = ((is_ParameterNode n))"
+
+fun is_FloatingNode :: "IRNode \<Rightarrow> bool" where
+  "is_FloatingNode n = ((is_AbstractLocalNode n) \<or> (is_BinaryNode n) \<or> (is_ConditionalNode n) \<or> (is_ConstantNode n) \<or> (is_FloatingGuardedNode n) \<or> (is_LogicNode n) \<or> (is_PhiNode n) \<or> (is_ProxyNode n) \<or> (is_UnaryNode n))"
+
+fun is_CallTargetNode :: "IRNode \<Rightarrow> bool" where
+  "is_CallTargetNode n = ((is_MethodCallTargetNode n))"
+
+fun is_ValueNode :: "IRNode \<Rightarrow> bool" where
+  "is_ValueNode n = ((is_CallTargetNode n) \<or> (is_FixedNode n) \<or> (is_FloatingNode n))"
+
+fun is_VirtualState :: "IRNode \<Rightarrow> bool" where
+  "is_VirtualState n = ((is_FrameState n))"
+
+fun is_Node :: "IRNode \<Rightarrow> bool" where
+  "is_Node n = ((is_ValueNode n) \<or> (is_VirtualState n))"
+
+fun is_MemoryKill :: "IRNode \<Rightarrow> bool" where
+  "is_MemoryKill n = ((is_AbstractMemoryCheckpoint n))"
+
+fun is_NarrowableArithmeticNode :: "IRNode \<Rightarrow> bool" where
+  "is_NarrowableArithmeticNode n = ((is_AbsNode n) \<or> (is_AddNode n) \<or> (is_AndNode n) \<or> (is_MulNode n) \<or> (is_NegateNode n) \<or> (is_NotNode n) \<or> (is_OrNode n) \<or> (is_SubNode n) \<or> (is_XorNode n))"
+
+fun is_AnchoringNode :: "IRNode \<Rightarrow> bool" where
+  "is_AnchoringNode n = ((is_AbstractBeginNode n))"
+
+fun is_DeoptBefore :: "IRNode \<Rightarrow> bool" where
+  "is_DeoptBefore n = ((is_DeoptimizingFixedWithNextNode n))"
+
+fun is_IndirectCanonicalization :: "IRNode \<Rightarrow> bool" where
+  "is_IndirectCanonicalization n = ((is_LogicNode n))"
+
+fun is_IterableNodeType :: "IRNode \<Rightarrow> bool" where
+  "is_IterableNodeType n = ((is_AbstractBeginNode n) \<or> (is_AbstractMergeNode n) \<or> (is_FrameState n) \<or> (is_IfNode n) \<or> (is_IntegerDivRemNode n) \<or> (is_InvokeWithExceptionNode n) \<or> (is_LoopBeginNode n) \<or> (is_LoopExitNode n) \<or> (is_MethodCallTargetNode n) \<or> (is_ParameterNode n) \<or> (is_ReturnNode n) \<or> (is_ShortCircuitOrNode n))"
+
+fun is_Invoke :: "IRNode \<Rightarrow> bool" where
+  "is_Invoke n = ((is_InvokeNode n) \<or> (is_InvokeWithExceptionNode n))"
+
+fun is_Proxy :: "IRNode \<Rightarrow> bool" where
+  "is_Proxy n = ((is_ProxyNode n))"
+
+fun is_ValueProxy :: "IRNode \<Rightarrow> bool" where
+  "is_ValueProxy n = ((is_PiNode n) \<or> (is_ValueProxyNode n))"
+
+fun is_ValueNodeInterface :: "IRNode \<Rightarrow> bool" where
+  "is_ValueNodeInterface n = ((is_ValueNode n))"
+
+fun is_ArrayLengthProvider :: "IRNode \<Rightarrow> bool" where
+  "is_ArrayLengthProvider n = ((is_AbstractNewArrayNode n) \<or> (is_ConstantNode n))"
+
+fun is_StampInverter :: "IRNode \<Rightarrow> bool" where
+  "is_StampInverter n = ((is_NegateNode n) \<or> (is_NotNode n))"
+
+fun is_GuardingNode :: "IRNode \<Rightarrow> bool" where
+  "is_GuardingNode n = ((is_AbstractBeginNode n))"
+
+fun is_SingleMemoryKill :: "IRNode \<Rightarrow> bool" where
+  "is_SingleMemoryKill n = ((is_BytecodeExceptionNode n) \<or> (is_ExceptionObjectNode n) \<or> (is_InvokeNode n) \<or> (is_InvokeWithExceptionNode n) \<or> (is_KillingBeginNode n) \<or> (is_StartNode n))"
+
+fun is_LIRLowerable :: "IRNode \<Rightarrow> bool" where
+  "is_LIRLowerable n = ((is_AbstractBeginNode n) \<or> (is_AbstractEndNode n) \<or> (is_AbstractMergeNode n) \<or> (is_BinaryOpLogicNode n) \<or> (is_CallTargetNode n) \<or> (is_ConditionalNode n) \<or> (is_ConstantNode n) \<or> (is_IfNode n) \<or> (is_InvokeNode n) \<or> (is_InvokeWithExceptionNode n) \<or> (is_IsNullNode n) \<or> (is_LoopBeginNode n) \<or> (is_PiNode n) \<or> (is_ReturnNode n) \<or> (is_SignedDivNode n) \<or> (is_SignedRemNode n) \<or> (is_UnaryOpLogicNode n) \<or> (is_UnwindNode n))"
+
+fun is_GuardedNode :: "IRNode \<Rightarrow> bool" where
+  "is_GuardedNode n = ((is_FloatingGuardedNode n))"
+
+fun is_ArithmeticLIRLowerable :: "IRNode \<Rightarrow> bool" where
+  "is_ArithmeticLIRLowerable n = ((is_AbsNode n) \<or> (is_BinaryArithmeticNode n) \<or> (is_NotNode n) \<or> (is_UnaryArithmeticNode n))"
+
+fun is_SwitchFoldable :: "IRNode \<Rightarrow> bool" where
+  "is_SwitchFoldable n = ((is_IfNode n))"
+
+fun is_VirtualizableAllocation :: "IRNode \<Rightarrow> bool" where
+  "is_VirtualizableAllocation n = ((is_NewArrayNode n) \<or> (is_NewInstanceNode n))"
+
+fun is_Unary :: "IRNode \<Rightarrow> bool" where
+  "is_Unary n = ((is_LoadFieldNode n) \<or> (is_LogicNegationNode n) \<or> (is_UnaryNode n) \<or> (is_UnaryOpLogicNode n))"
+
+fun is_FixedNodeInterface :: "IRNode \<Rightarrow> bool" where
+  "is_FixedNodeInterface n = ((is_FixedNode n))"
+
+fun is_BinaryCommutative :: "IRNode \<Rightarrow> bool" where
+  "is_BinaryCommutative n = ((is_AddNode n) \<or> (is_AndNode n) \<or> (is_IntegerEqualsNode n) \<or> (is_MulNode n) \<or> (is_OrNode n) \<or> (is_XorNode n))"
+
+fun is_Canonicalizable :: "IRNode \<Rightarrow> bool" where
+  "is_Canonicalizable n = ((is_BytecodeExceptionNode n) \<or> (is_ConditionalNode n) \<or> (is_DynamicNewArrayNode n) \<or> (is_PhiNode n) \<or> (is_PiNode n) \<or> (is_ProxyNode n) \<or> (is_StoreFieldNode n) \<or> (is_ValueProxyNode n))"
+
+fun is_UncheckedInterfaceProvider :: "IRNode \<Rightarrow> bool" where
+  "is_UncheckedInterfaceProvider n = ((is_InvokeNode n) \<or> (is_InvokeWithExceptionNode n) \<or> (is_LoadFieldNode n) \<or> (is_ParameterNode n))"
+
+fun is_Binary :: "IRNode \<Rightarrow> bool" where
+  "is_Binary n = ((is_BinaryArithmeticNode n) \<or> (is_BinaryNode n) \<or> (is_BinaryOpLogicNode n) \<or> (is_CompareNode n) \<or> (is_FixedBinaryNode n) \<or> (is_ShortCircuitOrNode n))"
+
+fun is_ArithmeticOperation :: "IRNode \<Rightarrow> bool" where
+  "is_ArithmeticOperation n = ((is_BinaryArithmeticNode n) \<or> (is_UnaryArithmeticNode n))"
+
+fun is_ValueNumberable :: "IRNode \<Rightarrow> bool" where
+  "is_ValueNumberable n = ((is_FloatingNode n) \<or> (is_ProxyNode n))"
+
+fun is_Lowerable :: "IRNode \<Rightarrow> bool" where
+  "is_Lowerable n = ((is_AbstractNewObjectNode n) \<or> (is_AccessFieldNode n) \<or> (is_BytecodeExceptionNode n) \<or> (is_ExceptionObjectNode n) \<or> (is_IntegerDivRemNode n) \<or> (is_UnwindNode n))"
+
+fun is_Virtualizable :: "IRNode \<Rightarrow> bool" where
+  "is_Virtualizable n = ((is_IsNullNode n) \<or> (is_LoadFieldNode n) \<or> (is_PiNode n) \<or> (is_StoreFieldNode n) \<or> (is_ValueProxyNode n))"
+
+fun is_Simplifiable :: "IRNode \<Rightarrow> bool" where
+  "is_Simplifiable n = ((is_AbstractMergeNode n) \<or> (is_BeginNode n) \<or> (is_IfNode n) \<or> (is_LoopExitNode n) \<or> (is_MethodCallTargetNode n) \<or> (is_NewArrayNode n))"
+
+fun is_StateSplit :: "IRNode \<Rightarrow> bool" where
+  "is_StateSplit n = ((is_AbstractStateSplit n) \<or> (is_BeginStateSplitNode n) \<or> (is_StoreFieldNode n))"
+(* nodeout *)
+
+fun is_sequential_node :: "IRNode \<Rightarrow> bool" where
+  "is_sequential_node (StartNode _ _) = True" |
+  "is_sequential_node (BeginNode _) = True" |
+  "is_sequential_node (KillingBeginNode _) = True" |
+  "is_sequential_node (LoopBeginNode _ _ _ _) = True" |
+  "is_sequential_node (LoopExitNode _ _ _) = True" |
+  "is_sequential_node (MergeNode _ _ _) = True" |
+  "is_sequential_node (RefNode _) = True" |
+  "is_sequential_node _ = False"
+
+text \<open>
+The following convenience function is useful in determining if
+two IRNodes are of the same type irregardless of their edges.
+It will return true if both the node parameters are the same node class.
+\<close>
+
+(* nodeout: isabelle-compare-type *)
+fun is_same_ir_node_type :: "IRNode \<Rightarrow> IRNode \<Rightarrow> bool" where
+"is_same_ir_node_type n1 n2 = (
+  ((is_AbsNode n1) \<and> (is_AbsNode n2)) \<or>
+  ((is_AddNode n1) \<and> (is_AddNode n2)) \<or>
+  ((is_AndNode n1) \<and> (is_AndNode n2)) \<or>
+  ((is_BeginNode n1) \<and> (is_BeginNode n2)) \<or>
+  ((is_BytecodeExceptionNode n1) \<and> (is_BytecodeExceptionNode n2)) \<or>
+  ((is_ConditionalNode n1) \<and> (is_ConditionalNode n2)) \<or>
+  ((is_ConstantNode n1) \<and> (is_ConstantNode n2)) \<or>
+  ((is_DynamicNewArrayNode n1) \<and> (is_DynamicNewArrayNode n2)) \<or>
+  ((is_EndNode n1) \<and> (is_EndNode n2)) \<or>
+  ((is_ExceptionObjectNode n1) \<and> (is_ExceptionObjectNode n2)) \<or>
+  ((is_FrameState n1) \<and> (is_FrameState n2)) \<or>
+  ((is_IfNode n1) \<and> (is_IfNode n2)) \<or>
+  ((is_IntegerEqualsNode n1) \<and> (is_IntegerEqualsNode n2)) \<or>
+  ((is_IntegerLessThanNode n1) \<and> (is_IntegerLessThanNode n2)) \<or>
+  ((is_InvokeNode n1) \<and> (is_InvokeNode n2)) \<or>
+  ((is_InvokeWithExceptionNode n1) \<and> (is_InvokeWithExceptionNode n2)) \<or>
+  ((is_IsNullNode n1) \<and> (is_IsNullNode n2)) \<or>
+  ((is_KillingBeginNode n1) \<and> (is_KillingBeginNode n2)) \<or>
+  ((is_LoadFieldNode n1) \<and> (is_LoadFieldNode n2)) \<or>
+  ((is_LogicNegationNode n1) \<and> (is_LogicNegationNode n2)) \<or>
+  ((is_LoopBeginNode n1) \<and> (is_LoopBeginNode n2)) \<or>
+  ((is_LoopEndNode n1) \<and> (is_LoopEndNode n2)) \<or>
+  ((is_LoopExitNode n1) \<and> (is_LoopExitNode n2)) \<or>
+  ((is_MergeNode n1) \<and> (is_MergeNode n2)) \<or>
+  ((is_MethodCallTargetNode n1) \<and> (is_MethodCallTargetNode n2)) \<or>
+  ((is_MulNode n1) \<and> (is_MulNode n2)) \<or>
+  ((is_NegateNode n1) \<and> (is_NegateNode n2)) \<or>
+  ((is_NewArrayNode n1) \<and> (is_NewArrayNode n2)) \<or>
+  ((is_NewInstanceNode n1) \<and> (is_NewInstanceNode n2)) \<or>
+  ((is_NotNode n1) \<and> (is_NotNode n2)) \<or>
+  ((is_OrNode n1) \<and> (is_OrNode n2)) \<or>
+  ((is_ParameterNode n1) \<and> (is_ParameterNode n2)) \<or>
+  ((is_PiNode n1) \<and> (is_PiNode n2)) \<or>
+  ((is_ReturnNode n1) \<and> (is_ReturnNode n2)) \<or>
+  ((is_ShortCircuitOrNode n1) \<and> (is_ShortCircuitOrNode n2)) \<or>
+  ((is_SignedDivNode n1) \<and> (is_SignedDivNode n2)) \<or>
+  ((is_StartNode n1) \<and> (is_StartNode n2)) \<or>
+  ((is_StoreFieldNode n1) \<and> (is_StoreFieldNode n2)) \<or>
+  ((is_SubNode n1) \<and> (is_SubNode n2)) \<or>
+  ((is_UnwindNode n1) \<and> (is_UnwindNode n2)) \<or>
+  ((is_ValuePhiNode n1) \<and> (is_ValuePhiNode n2)) \<or>
+  ((is_ValueProxyNode n1) \<and> (is_ValueProxyNode n2)) \<or>
+  ((is_XorNode n1) \<and> (is_XorNode n2)))"
+
+end
